move label definitions in ….Stateful, simplify NSL labels (Fabian's remark)

examples/nsl_pk/DY.Example.NSL.Protocol.Stateful.fst
@@ -51,6 +51,20 @@ instance event_nsl_event: event nsl_event = {
   format = mk_parseable_serializeable ps_nsl_event;
 }
 
+(*** Labels used to generate randomness ***)
+
+val long_term_decryption_key_label:
+  principal ->
+  label
+let long_term_decryption_key_label prin =
+  principal_tag_label prin "DY.Lib.State.PrivateKeys"
+
+val nsl_nonce_label:
+  principal ->
+  label
+let nsl_nonce_label prin =
+  principal_label prin
+
 (*** Stateful code ***)
 
 type nsl_global_sess_ids = {
@@ -60,11 +74,7 @@ type nsl_global_sess_ids = {
 
 val prepare_msg1: principal -> principal -> traceful state_id
 let prepare_msg1 alice bob =
-  let* n_a = mk_rand NoUsage (
-    join
-      (join (principal_tag_label alice "DY.Lib.State.PrivateKeys") (principal_tag_label alice "NSL.Session"))
-      (join (principal_tag_label bob "DY.Lib.State.PrivateKeys") (principal_tag_label bob "NSL.Session"))
-  ) 32 in
+  let* n_a = mk_rand NoUsage (join (nsl_nonce_label alice) (nsl_nonce_label bob)) 32 in
   trigger_event alice (Initiate1 alice bob n_a);*
   let* sess_id = new_session_id alice in
   set_state alice sess_id (InitiatorSentMsg1 bob n_a <: nsl_session);*
@@ -76,7 +86,7 @@ let send_msg1 global_sess_id alice sess_id =
   match st with
   | InitiatorSentMsg1 bob n_a -> (
     let*? pk_b = get_public_key alice global_sess_id.pki (PkEnc "NSL.PublicKey") bob in
-    let* nonce = mk_rand PkNonce (principal_tag_label alice "DY.Lib.State.PrivateKeys") 32 in
+    let* nonce = mk_rand PkNonce (long_term_decryption_key_label alice) 32 in
     let msg = compute_message1 alice bob pk_b n_a nonce in
     let* msg_id = send_msg msg in
     return (Some msg_id)
@@ -88,11 +98,7 @@ let prepare_msg2 global_sess_id bob msg_id =
   let*? msg = recv_msg msg_id in
   let*? sk_b = get_private_key bob global_sess_id.private_keys (PkDec "NSL.PublicKey") in
   let*? msg1: message1 = return (decode_message1 bob msg sk_b) in
-  let* n_b = mk_rand NoUsage (
-    join
-      (join (principal_tag_label msg1.alice "DY.Lib.State.PrivateKeys") (principal_tag_label msg1.alice "NSL.Session"))
-      (join (principal_tag_label bob "DY.Lib.State.PrivateKeys") (principal_tag_label bob "NSL.Session"))
-  ) 32 in
+  let* n_b = mk_rand NoUsage (join (nsl_nonce_label msg1.alice) (nsl_nonce_label bob)) 32 in
   trigger_event bob (Respond1 msg1.alice bob msg1.n_a n_b);*
   let* sess_id = new_session_id bob in
   set_state bob sess_id (ResponderSentMsg2 msg1.alice msg1.n_a n_b <: nsl_session);*
@@ -104,7 +110,7 @@ let send_msg2 global_sess_id bob sess_id =
   match st with
   | ResponderSentMsg2 alice n_a n_b -> (
     let*? pk_a = get_public_key bob global_sess_id.pki (PkEnc "NSL.PublicKey") alice in
-    let* nonce = mk_rand PkNonce (principal_tag_label bob "DY.Lib.State.PrivateKeys") 32 in
+    let* nonce = mk_rand PkNonce (long_term_decryption_key_label bob) 32 in
     let msg = compute_message2 bob {n_a; alice;} pk_a n_b nonce in
     let* msg_id = send_msg msg in
     return (Some msg_id)
@@ -131,7 +137,7 @@ let send_msg3 global_sess_id alice sess_id =
   match st with
   | InitiatorSentMsg3 bob n_a n_b -> (
     let*? pk_b = get_public_key alice global_sess_id.pki (PkEnc "NSL.PublicKey") bob in
-    let* nonce = mk_rand PkNonce (principal_tag_label alice "DY.Lib.State.PrivateKeys") 32 in
+    let* nonce = mk_rand PkNonce (long_term_decryption_key_label alice) 32 in
     let msg = compute_message3 alice bob pk_b n_b nonce in
     let* msg_id = send_msg msg in
     return (Some msg_id)
