examples/iso_dh/DY.Example.DH.Protocol.Total.Proof.fst
@@ -10,18 +10,6 @@ open DY.Example.DH.Protocol.Stateful
 
 (*** Cryptographic invariants ***)
 
-val long_signature_key_label:
-  principal ->
-  label
-let long_signature_key_label prin =
-  principal_tag_label prin "DY.Lib.State.PrivateKeys"
-
-val ephemeral_dh_key_label:
-  principal -> state_id ->
-  label
-let ephemeral_dh_key_label prin sess_id =
-  principal_tagged_state_label prin sess_id "DH.Session"
-
 val dh_crypto_usages: crypto_usages
 instance dh_crypto_usages = {
   default_crypto_usages with
@@ -50,7 +38,7 @@ let dh_crypto_preds = {
   sign_pred = {
     pred = (fun tr vk sig_msg ->
       get_signkey_usage vk == SigKey "DH.SigningKey" empty /\
-      (exists prin. get_signkey_label tr vk == long_signature_key_label prin /\ (
+      (exists prin. get_signkey_label tr vk == long_term_signature_key_label prin /\ (
         match parse sig_message sig_msg with
         | Some (SigMsg2 sig_msg2) -> (
           exists y. sig_msg2.gy == (dh_pk y) /\ event_triggered tr prin (Respond1 sig_msg2.alice prin sig_msg2.gx sig_msg2.gy y)
@@ -142,8 +130,8 @@ val compute_message2_proof:
     event_triggered tr bob (Respond1 alice bob gx (dh_pk y) y) /\
     is_publishable tr gx /\
     bytes_invariant tr y /\
-    is_signature_key (SigKey "DH.SigningKey" empty) (long_signature_key_label bob) tr sk_b /\
-    is_secret (long_signature_key_label bob) tr n_sig /\
+    is_signature_key (SigKey "DH.SigningKey" empty) (long_term_signature_key_label bob) tr sk_b /\
+    is_secret (long_term_signature_key_label bob) tr n_sig /\
     SigNonce? (get_usage n_sig)
   )
   (ensures
@@ -187,20 +175,20 @@ val decode_and_verify_message2_proof:
   (requires
     is_publishable tr msg2_bytes /\
     is_secret (ephemeral_dh_key_label alice alice_si) tr x /\
-    is_verification_key (SigKey "DH.SigningKey" empty) (long_signature_key_label bob) tr pk_b
+    is_verification_key (SigKey "DH.SigningKey" empty) (long_term_signature_key_label bob) tr pk_b
   )
   (ensures (
     match decode_and_verify_message2 msg2_bytes alice x pk_b with
     | Some res -> (
       let sig_msg = SigMsg2 {alice; gx=(dh_pk x); gy=res.gy} in
       is_publishable tr res.gy /\
-      (is_corrupt tr (long_signature_key_label bob) \/
+      (is_corrupt tr (long_term_signature_key_label bob) \/
       (exists y. event_triggered tr bob (Respond1 alice bob (dh_pk x) res.gy y)))
     )
     | None -> True
   ))
 let decode_and_verify_message2_proof tr msg2_bytes alice alice_si bob x pk_b =
-  assume(forall p. (long_signature_key_label bob) == (long_signature_key_label p) ==> bob == p);
+  assume(forall p. (long_term_signature_key_label bob) == (long_term_signature_key_label p) ==> bob == p);
   match decode_and_verify_message2 msg2_bytes alice x pk_b with
     | Some res -> (
       parse_wf_lemma message (is_publishable tr) msg2_bytes;
@@ -213,7 +201,7 @@ let decode_and_verify_message2_proof tr msg2_bytes alice alice_si bob x pk_b =
       assert(is_publishable tr res.gy);
       
       assert(
-        is_corrupt tr (long_signature_key_label bob) \/
+        is_corrupt tr (long_term_signature_key_label bob) \/
         (exists y. res.gy == dh_pk y /\ event_triggered tr bob (Respond1 alice bob gx gy y))
       );
       ()
@@ -231,8 +219,8 @@ val compute_message3_proof:
     event_triggered tr alice (Initiate2 alice bob (dh_pk x) gy (dh x gy)) /\
     is_publishable tr gx /\ is_publishable tr gy /\
     gx = dh_pk x /\
-    is_signature_key (SigKey "DH.SigningKey" empty) (long_signature_key_label alice) tr sk_a /\
-    is_secret (long_signature_key_label alice) tr n_sig /\
+    is_signature_key (SigKey "DH.SigningKey" empty) (long_term_signature_key_label alice) tr sk_a /\
+    is_secret (long_term_signature_key_label alice) tr n_sig /\
     SigNonce? (get_usage n_sig)
   )
   (ensures
@@ -272,20 +260,20 @@ val decode_and_verify_message3_proof:
     is_publishable tr msg3_bytes /\
     is_publishable tr gx /\
     is_secret (ephemeral_dh_key_label bob bob_si) tr y /\
-    is_verification_key (SigKey "DH.SigningKey" empty) (long_signature_key_label alice) tr pk_a
+    is_verification_key (SigKey "DH.SigningKey" empty) (long_term_signature_key_label alice) tr pk_a
   )
   (ensures (
     let gy = dh_pk y in
     match decode_and_verify_message3 msg3_bytes bob gx gy y pk_a with
     | Some res -> (
       let sig_msg = SigMsg3 {bob; gx; gy} in
-      (is_corrupt tr (long_signature_key_label alice) \/
+      (is_corrupt tr (long_term_signature_key_label alice) \/
       (exists x. gx == dh_pk x /\ event_triggered tr alice (Initiate2 alice bob gx gy (dh x gy))))
     )
     | None -> True
   ))
 let decode_and_verify_message3_proof tr msg3_bytes alice bob bob_si gx y pk_a =
-  assume(forall p. (long_signature_key_label alice) == (long_signature_key_label p) ==> alice == p);
+  assume(forall p. (long_term_signature_key_label alice) == (long_term_signature_key_label p) ==> alice == p);
   let gy = dh_pk y in
   match decode_and_verify_message3 msg3_bytes bob gx gy y pk_a with
     | Some res -> (
