examples/iso_dh/DY.Example.DH.SecurityProperties.fst
@@ -22,7 +22,7 @@ val responder_authentication:
     event_triggered_at tr i alice (Initiate2 alice bob gx gy k)
   )
   (ensures 
-    is_corrupt (prefix tr i) (long_signature_key_label bob) \/
+    is_corrupt (prefix tr i) (long_term_signature_key_label bob) \/
     (exists y. event_triggered (prefix tr i) bob (Respond1 alice bob gx gy y) /\
     k == dh y gx)
   )
@@ -38,7 +38,7 @@ val initiator_authentication:
     event_triggered_at tr i bob (Respond2 alice bob gx gy k)
   )
   (ensures 
-    is_corrupt (prefix tr i) (long_signature_key_label alice) \/
+    is_corrupt (prefix tr i) (long_term_signature_key_label alice) \/
     event_triggered (prefix tr i) alice (Initiate2 alice bob gx gy k)
   )
 let initiator_authentication tr i alice bob gx gy k = ()
@@ -54,7 +54,7 @@ val initiator_forward_secrecy:
     attacker_knows tr k
   )
   (ensures
-    is_corrupt tr (long_signature_key_label bob) \/
+    is_corrupt tr (long_term_signature_key_label bob) \/
     (exists bob_si. is_corrupt tr (ephemeral_dh_key_label bob bob_si)) \/
     is_corrupt tr (ephemeral_dh_key_label alice alice_si)
   )
@@ -67,7 +67,7 @@ let initiator_forward_secrecy tr alice alice_si bob gx gy k =
   assert(
     (exists x. gx == dh_pk x /\ k == dh x gy /\ is_secret (ephemeral_dh_key_label alice alice_si) tr x) /\
     (
-      is_corrupt tr (long_signature_key_label bob) \/
+      is_corrupt tr (long_term_signature_key_label bob) \/
       (exists y.
         (exists bob_si. is_secret (ephemeral_dh_key_label bob bob_si) tr y) /\
         gy = dh_pk y
@@ -78,14 +78,14 @@ let initiator_forward_secrecy tr alice alice_si bob gx gy k =
   // We can deduce from it the label of `k`, up to some corruption
   // (this assert is not needed and only there for pedagogical purposes)
   assert(
-    is_corrupt tr (long_signature_key_label bob) \/
+    is_corrupt tr (long_term_signature_key_label bob) \/
     (exists bob_si. get_label tr k == join (ephemeral_dh_key_label alice alice_si) (ephemeral_dh_key_label bob bob_si))
   );
 
   // We deduce from the following this assertion,
   // that will trigger transitivity of `can_flow tr` from `join ...` to `get_label k` to `public`
   assert(
-    is_corrupt tr (long_signature_key_label bob) \/
+    is_corrupt tr (long_term_signature_key_label bob) \/
     (exists bob_si. join (ephemeral_dh_key_label alice alice_si) (ephemeral_dh_key_label bob bob_si) `can_flow tr` public)
   );
 
@@ -103,7 +103,7 @@ val responder_forward_secrecy:
     attacker_knows tr k
   )
   (ensures
-    is_corrupt tr (long_signature_key_label alice) \/
+    is_corrupt tr (long_term_signature_key_label alice) \/
     (exists alice_si. is_corrupt tr (ephemeral_dh_key_label alice alice_si)) \/
     is_corrupt tr (ephemeral_dh_key_label bob bob_si)
   )
@@ -116,7 +116,7 @@ let responder_forward_secrecy tr alice bob bob_si gx gy k =
   assert(
     (exists y. gy == dh_pk y /\ k == dh y gx /\ is_secret (ephemeral_dh_key_label bob bob_si) tr y) /\
     (
-      is_corrupt tr (long_signature_key_label alice) \/
+      is_corrupt tr (long_term_signature_key_label alice) \/
       (exists x.
         (exists alice_si. is_secret (ephemeral_dh_key_label alice alice_si) tr x) /\
         k == dh x gy
@@ -127,21 +127,21 @@ let responder_forward_secrecy tr alice bob bob_si gx gy k =
   // We can deduce from it the label of `k`, up to some corruption
   // (this assert is not needed and only there for pedagogical purposes)
   assert(
-    is_corrupt tr (long_signature_key_label alice) \/
+    is_corrupt tr (long_term_signature_key_label alice) \/
     (exists alice_si. get_label tr k == join (ephemeral_dh_key_label alice alice_si) (ephemeral_dh_key_label bob bob_si))
   );
 
   // We deduce from the following this assertion,
   // that will trigger transitivity of `can_flow tr` from `join ...` to `get_label k` to `public`
   assert(
-    is_corrupt tr (long_signature_key_label alice) \/
+    is_corrupt tr (long_term_signature_key_label alice) \/
     (exists alice_si. join (ephemeral_dh_key_label alice alice_si) (ephemeral_dh_key_label bob bob_si) `can_flow tr` public)
   );
 
   // This assert is needed for the proof
   assert(exists alice_si. join (ephemeral_dh_key_label alice alice_si) (ephemeral_dh_key_label bob bob_si)
     `can_flow tr` public \/ 
-    is_corrupt tr (long_signature_key_label alice));
+    is_corrupt tr (long_term_signature_key_label alice));
 
   // This assert allows to deduce corruption of principal alice from corruption state alice_si of principal alice
   assert(forall alice_si. principal_label alice `can_flow tr` ephemeral_dh_key_label alice alice_si);
